\documentclass[12pt]{article}
\usepackage{techart}
\begin{document}
\title{STAT 651 HW 4 Solution}
\author{}\date{}
\maketitle

\begin{enumerate}
\item (12 pts)

\begin{enumerate}
\item Check the three properties: (1) 0, 1; (2) non-decreasing; (3)
right-continuous.

\item
Find the inverse of the cdf:
\[
F^{-1}(y) = \tan\bigl((y - 1/2)\pi\bigr)
\]
By theorem~2.1.10, randomly draw $y$ from uniform on $(0, 1)$,
then $X = F^{-1}(y)$ is a random draw of $X$.
\end{enumerate}

\item (24 pts)

\begin{enumerate}
\item
$y = g(x) = x^3$, $x = g^{-1}(y) = y^{1/3}$.
\[
f_Y(y)
= f_X\bigl(g^{-1}(y)\bigr)
    \biggl|\frac{\diff g^{-1}(y)}{\diff y}\biggr|
= 42 y^{5/3} (1 - y^{1/3}) \cdot \frac{1}{3} y^{-2/3}
= 14 y(1 - y^{1/3})
,\quad
0 < y < 1
\]
\[
\int_0^1 f_X(x) \diff x
= \int_0^1 42 x^5(1 - x) \diff x
= \int_0^1 42x^5 \diff x - \int_0^1 42 x^6 \diff x
= \int_0^1 7 \diff x^6 - \int_0^1 6 \diff x^7
= 1
\]
\[
\int_0^1 f_Y(y)
= \int_0^1 14y(1 - y^{1/3}) \diff y
= \int_0^1 14y \diff y - \int_0^1 14 y^{4/3} \diff y
= \int_0^1 7\diff y^2 - \int_0^1 14\frac{3}{7} \diff y^{7/3}
= 1
\]

\item
$y = g(x) = 4x + 3$,
$x = g^{-1}(y) = \frac{y-3}{4}$.
\[
f_Y(y)
= f_X\bigl(g^{-1}(y)\bigr) \biggl|\frac{\diff g^{-1}(y)}{\diff y}\biggr|
= 7 \exp\Bigl(-7\frac{y-3}{4}\Bigr) \frac{1}{4}
= \frac{7}{4} \exp\Bigl(-\frac{7}{4}y + \frac{21}{4}\Bigr)
,\quad
3 < y < \infty
\]
\[
\int_0^\infty f_X(x) \diff x
= \int_0^\infty 7\exp(-7x) \diff x
= -e^{-7x}\Bigm|_0^\infty
= 1
\]
\[
\int_3^\infty f_Y(y) \diff y
= \int_3^\infty \frac{7}{4}\exp\Bigl(-\frac{7}{4}y + \frac{21}{4}\Bigr) \diff y
= -\exp\Bigl(-\frac{7}{4}y + \frac{21}{4}\Bigr) \Bigm|_3^\infty
= 1
\]
Note: always remember to indicate the range for the pdf definition.
\end{enumerate}

\item (14 pts)

$Y = X / (X + 1) = 1 - \frac{1}{X + 1}$,
$X = \frac{1}{1 - Y} - 1$.
Clearly, $X$ and $Y$ have a one-to-one correspondence.
\[
P(Y = y)
= P\Bigl(X = \frac{1}{1 - y} - 1\Bigr)
= \frac{1}{3} \Bigl(\frac{2}{3}\Bigr)^{\frac{1}{1-y} - 1}
= \frac{1}{2} \Bigl(\frac{2}{3}\Bigr)^{\frac{1}{1-y}}
,\quad
y = 0/1, 1/2, 2/3, 3/4,\dotso
\]

\item (24 pts)

(Graphs omitted.)

\begin{enumerate}
\item
Define $Z = |X|$, then
$f_Z(z) = \exp(-z)$, $0 \le z < \infty$.

Since
$y = g(z) = z^3$, $y \ge 0$,
we have
$z = g^{-1}(y) = y^{1/3}$, and
\[
f_Y(y)
= f_Z\bigl(g^{-1}(y)\bigr)
    \biggl|\frac{\diff g^{-1}(y)}{\diff y}\biggr|
= \frac{1}{3} y^{-2/3} e^{-y^{1/3}}
,\quad
y \ge 0
\]

\[
\int_0^\infty f_Y(y) \diff y
= \int_0^\infty e^{-y^{1/3}} \diff y^{1/3}
= -e^{-y^{1/3}} \biggm|_0^\infty
= 1
\]

(An alternative is to use Theorem~2.1.8 directly.
Actually the density if $Z$ is obtained following Theorem~2.1.8.
I had the solution above when I noticed that $f_X$ is a function of
$|X|$ where $Y$ is a monotone function of $|X|$, therefore
the problem is really about $|X|$, and $X$ can be skipped.)

\item
\[
y =
\begin{cases}
    g_1(x) = 1 - x^2, & x \ge 0\\
    g_2(x) = 1 - x^2, & x < 0
\end{cases}
\]
\[
x =
\begin{cases}
g_1^{-1}(y) = \sqrt{1 - y}, & x \ge 0\\
g_2^{-1}(y) = -\sqrt{1 - y}, & x < 0
\end{cases}
\]

\[
f_Y(y)
= f_X\bigl(g_1^{-1}(y)\bigr)
    \biggl|\frac{\diff g_1^{-1}(y)}{\diff y}\biggr|
+ f_X\bigl(g_2^{-1}(y)\bigr)
    \biggl|\frac{\diff g_2^{-1}(y)}{\diff y}\biggr|
= \frac{3}{8} \frac{2 - y}{\sqrt{1 - y}}
= \frac{3}{8}\biggl(\frac{1}{\sqrt{1 - y}} + \sqrt{1 - y}\biggr)
\]
$0 < y < 1$.

\[
\int_0^1 f_Y(y) \diff y
= \frac{3}{8} \int_0^1 \biggl(\frac{1}{\sqrt{1-y}} + \sqrt{1-y}\biggr)
    \diff y
= \frac{3}{8} \int_0^1 \biggl(\frac{1}{\sqrt{z}} + \sqrt{z}\biggr)
    \diff z
= \frac{3}{8}\biggl(2\sqrt{z} + \frac{2}{3} z^{3/2}\biggr)_0^1
= 1
\]
\end{enumerate}

\item (12 pts)

\[
E(X) = (.25)(-1) + (.10)(0) + (.45)(1) + (.2)(2) = 0.6
\]
\[
E(X^2) = (.25)(1) + (.10)(0) + (.45)(1) + (.2)(4) = 1.5
\]
\[
\var(X) = E(X^2) - \bigl(E(X)\bigr)^2 = 1.5 - 0.6^2 = 1.14
\]

\item (14 pts)

\begin{enumerate}
\item
\[
k = \biggl(\int_{-1}^1 (1 - x^2) \diff x\bigg)^{-1} = 3/4
\]

\item
\[
E(X)
= \int_{-1}^1 \frac{3}{4} x (1 - x^2) \diff x
= \frac{3}{4}\biggl(\frac{1}{2}x^2 - \frac{1}{4}x^4\biggr)_{-1}^1
= 0
\]
(If we noticed $f_X(x)$ is symmetric about 0,
this would be obvious.)
\[
E(X^2)
= \int_{-1}^1 \frac{3}{4} x^2 (1 - x^2) \diff x
= \frac{3}{4}\biggl(\frac{1}{3}x^3 - \frac{1}{5}x^5\biggr)_{-1}^1
= 1/5
\]
\[
\var(X) = E(X^2) - \bigl(E(X)\bigr)^2 = 1/5
\]

\end{enumerate}
\end{enumerate}


\end{document}
